# Exercise1

See [Liouville's theorem](https://en.wikipedia.org/wiki/Harmonic_function#Liouville's_theorem) and [Corollary 2.8](https://www.math.ucdavis.edu/~hunter/pdes/ch2.pdf#page=6).

# Exercise2

$\phi$ will be unbound if $\Delta \phi = c$.

# Exercise3

According to Stoke's theorem,
$$
\begin{aligned}
\int_\partial g \star df &= \int d(g \star df) = \int dg \wedge \star df + \int g \wedge d \star df \\
                         &= \int dg \wedge \star df + \int g \wedge \star  \Delta f \\
                         &= \langle \nabla g, \nabla f \rangle + \langle g, \Delta f \rangle
\end{aligned}
$$

On the other hand,
$$
\begin{aligned}
\int_\partial g \star df &= \langle g, N \cdot \nabla f \rangle_\partial
\end{aligned}
$$

Therefore,
$$
\begin{aligned}
\langle \Delta f, g \rangle &= -\langle \nabla f, \nabla g \rangle + \langle N \cdot \nabla f, g \rangle_\partial
\end{aligned}
$$

# Exercise4

When there's no boundary, accordingt to Greenâ€™s identity:

$$
\begin{aligned}
\langle \Delta f, g \rangle &= -\langle \nabla f, \nabla g \rangle
\end{aligned}
$$

Then,

$$
\begin{aligned}
\langle \Delta f, f \rangle &= -\langle \nabla f, \nabla f \rangle \leq 0
\end{aligned}
$$

Therefore, $\Delta$ is negative-semidefinite.

# Exercise5

$$
\begin{aligned}
w = w_1 + w_2 = h \cot{\alpha} + h \cot{\beta}
\end{aligned}
$$

Then,

$$
\begin{aligned}
\frac{w}{h} = \cot{\alpha} + \cot{\beta}
\end{aligned}
$$

# Exercise6

Since hat function $\phi$ is a linear function, we have $\phi(x) = \phi(x_0) + \nabla \phi \cdot (x - x_0)$. Then,

$$
\begin{aligned}
\phi(v_1) = 1
\end{aligned}
$$

$$
\begin{aligned}
\phi(v_2) = \phi(v_1) + \nabla \phi \cdot (v_2 - v_1) = 0 \\
\phi(v_3) = \phi(v_1) + \nabla \phi \cdot (v_3 - v_1) = 0
\end{aligned}
$$

Therefore, 

$$
\begin{aligned}
\phi(v_3) - \phi(v_2) = \nabla \phi \cdot (v_3 - v_2) = 0
\end{aligned}
$$

which means $\nabla \phi$ is perpendicular to the edge $e$, pointing to $v_1$. Next, plugging in the direction,

$$
\begin{aligned}
1 = \nabla \phi \cdot (v_1 - v_2) &= | \nabla \phi | \cdot | v_1 - v_2 | \cos{\theta} \\
                                  &= | \nabla \phi | \cdot h
\end{aligned}
$$

$$
\begin{aligned}
| \nabla \phi | = \frac{1}{h} = \frac{w}{w h} = \frac{w}{2 A}
\end{aligned}
$$

which means the norm of $\phi$ equals to $\frac{w}{2 A}$, where $w$ is the length of edge $e$. Putting everything together, we have

$$
\begin{aligned}
\nabla \phi = \frac{e^{\perp}}{2 A}
\end{aligned}
$$

Also see [Cotan Laplacian](https://graphics.stanford.edu/courses/cs468-13-spring/assets/lecture12-lu.pdf#page=4).

# Exercise7

$$
\begin{aligned}
\langle \nabla \phi, \nabla \phi \rangle &= \int_A \nabla \phi \cdot \nabla \phi \ d \sigma \\
                                         &= \int_A \frac{1}{h^2} \ d \sigma \\
                                         &= \frac{A}{h^2} \\
                                         &= \frac{w}{2 h} \\
                                         &= \frac{1}{2} (\cot{\alpha} + \cot{\beta})
\end{aligned}
$$

# Exercise8

$$
\begin{aligned}
\langle \nabla \phi_i, \nabla \phi_j \rangle &= \int_A \nabla \phi_i \cdot \nabla \phi_j \ d \sigma \\
                                             &= \int_A \frac{e_i^{\perp}}{2 A} \cdot \frac{e_j^{\perp}}{2 A} \ d \sigma \\
                                             &= \frac{e_i \cdot e_j}{4A^2} \cdot A \\
                                             &= \frac{e_i \cdot e_j}{4 A} \\
                                             &= \frac{|e_i| |e_j| \cos{(\pi - \theta)}}{2 |e_i| |e_j| \sin{(\pi - \theta)}} \\
                                             &= \frac{-\cos{\theta}}{2 \sin{\theta}} \\
                                             &= -\frac{1}{2} \cot{\theta}
\end{aligned}
$$

# Exercise9

$$
\begin{aligned}
\frac{|e_{ij}^\star|}{|e_{ij}|} &= \frac{|e_{1}^\star| + |e_{2}^\star|}{|e_{ij}|} = \frac{|e_{1}^\star|}{|e_{ij}|} + \frac{|e_{2}^\star|}{|e_{ij}|} \\
                                &= \frac{\frac{1}{2} |e_{ij}| \cot{\alpha}}{|e_{ij}|} + \frac{\frac{1}{2} |e_{ij}| \cot{\beta}}{|e_{ij}|} \\
                                &= \frac{1}{2} (\cot{\alpha} + \cot{\beta})
\end{aligned}
$$
