# Exercise1

$\forall u \in U, v \in \text{ker}(A^*)$, we have

$$
\langle \langle A u, v \rangle \rangle = \langle \langle u, A^* v \rangle \rangle = 0
$$

$$
v \in \text{im}(A)^\perp \Rightarrow \text{ker}(A^*) \subset \text{coker}(A)
$$

Similarly, $\forall u \in U, v \in \text{coker}(A)$ we have

$$
\langle \langle u, A^* v \rangle \rangle = \langle \langle A u, v \rangle \rangle = 0
$$

$$
A^* v = 0 \Rightarrow \text{coker}(A) \subset \text{ker}(A^*)
$$

Therefore,

$$
\text{coker}(A) = \text{ker}(A^*)
$$

# Exercise2

First prove that $(A^*)^* = A$. $\forall u \in U, v \in V$, we have

$$
\langle \langle A^* v, u \rangle \rangle = \langle \langle u, A^* v \rangle \rangle = \langle \langle A u, v \rangle \rangle = \langle \langle v, A u \rangle \rangle
$$

$$
(A^*)^* = A
$$

Then, 

$$
(B \circ A) u = 0 \Rightarrow A u \in \text{ker}(B) = \text{coker}(B^*) = \text{im}(B^*)^\perp
$$

$$
\text{im}(A) \cap \text{im}(B^*) = 0
$$

# Exercise3

First decompose $v$ into $\text{im}(A)$ and $\text{coker}(A)$:

$$
v = A u + v' \\
$$

where $u \in U$ and $v' \in \text{coker}(A)=\text{ker}(A^*)$. Then, decompose $v'$ with $B^*$:

$$
v' = B^* w + z \\
$$

where $w \in W$ and $z \in \text{coker}(B^*)=\text{ker}(B)$. 

Furthermore,

$$
A^* v' = A^* B^* w + A^* z = 0 \\
$$

Since $\forall u \in U$ and $\forall w \in W$, we have:

$$
\begin{aligned}
\langle \langle A u, B^* w \rangle \rangle &= \langle \langle u, A^* B^* w \rangle \rangle \\
&= \langle \langle B A u, w \rangle \rangle = 0 
\end{aligned}
$$

Then, 

$$
A^* B^* w = 0
$$

and

$$
A^* z = -A^* B^* w = 0
$$

which means $z \in \text{ker}(A^*)$ and $z \in \text{ker}(B)$.

Therefore,

$$
v = A u + B^* w + z \\
$$

# Exercise4

$$
\begin{aligned}
\int_M d (\alpha \wedge \star \beta) &= \int_M d \alpha \wedge \star \beta + \int_M (-1)^k \alpha \wedge d \star \beta \\
&= \langle \langle d \alpha, \beta \rangle \rangle - \langle \langle \alpha, \delta \beta \rangle \rangle \\
&= \int_{\partial M} \alpha \wedge \star \beta =  0
\end{aligned}
$$

Therefore, 

$$
\begin{aligned}
\langle \langle d \alpha, \beta \rangle \rangle = \langle \langle \alpha, \delta \beta \rangle \rangle
\end{aligned}
$$

Also see [Hodge star operator-Codifferential](https://en.wikipedia.org/wiki/Hodge_star_operator#Codifferential).

# Exercise5

From [Exercise4](#exercise4) we know that $d$ and $\delta$ are adjoint. Since $d \circ d$ is a chain complex, we have

$$
\begin{aligned}
\omega = d \alpha + \delta \beta + \gamma
\end{aligned}
$$

where $\alpha$ is a ($k$-1)-form, $\beta$ is a ($k$+1)-form, $\gamma$ is a $k$-form such that $d \gamma = 0$ and $\delta \gamma = 0$.

# Exercise6

$$
\begin{aligned}
\delta \beta &= \star d \star \beta = \star d \star \star \phi \\
&= \star d \phi \\
&= \star (\nabla \phi)^\flat \\
&= ((\nabla \phi)^\perp)^\flat
\end{aligned}
$$

# Exercise7

When $\gamma$ is harmonic, we have

$$
\begin{aligned}
\Delta \gamma = d \delta \gamma + \delta d \gamma = d (0) + \delta (0) = 0
\end{aligned}
$$

When $\Delta \gamma = 0$, we have

$$
\begin{aligned}
\Delta \gamma = d \delta \gamma + \delta d \gamma = 0
\end{aligned}
$$

Let $d \alpha$ be a $k$-form, then

$$
\begin{aligned}
\langle \langle \Delta \gamma, d \alpha \rangle \rangle &= \langle \langle d \delta \gamma + \delta d \gamma, d \alpha \rangle \rangle \\
&= \langle \langle d \delta \gamma, d \alpha \rangle \rangle + \langle \langle \delta d \gamma, d \alpha \rangle \rangle \\
&= \langle \langle \delta \gamma, \delta d \alpha \rangle \rangle + \langle \langle d \gamma, d d \alpha \rangle \rangle \\
&= \langle \langle \delta \gamma, \delta d \alpha \rangle \rangle \\
&= 0
\end{aligned}
$$

We must have $\delta \gamma = 0$. Similarly, let $\delta \beta$ be a $k$-form,

$$
\begin{aligned}
\langle \langle \Delta \gamma, \delta \beta \rangle \rangle &= \langle \langle d \delta \gamma + \delta d \gamma, \delta \beta \rangle \rangle \\
&= \langle \langle d \delta \gamma, \delta \beta \rangle \rangle + \langle \langle \delta d \gamma, \delta \beta \rangle \rangle \\
&= \langle \langle d d \delta \gamma, \beta \rangle \rangle + \langle \langle d \gamma, \delta d \beta \rangle \rangle \\
&= \langle \langle d \gamma, \delta d \beta \rangle \rangle \\
&= 0
\end{aligned}
$$

We must have $d \gamma = 0$, which means $\gamma$ is harmonic.

Therefore, $\gamma$ is harmonic if and only if $\Delta \gamma = 0$.

# Exercise8

From [Exercise1](#exercise1) we know that $\text{coker}(A) = \text{ker}(A^*)$, therefore,

$$
\begin{aligned}
\text{im}(A) \cap \text{ker}(A^*) = \text{im}(A) \cap \text{coker}(A) = 0
\end{aligned}
$$

# Exercise9

From [Exercise5](#exercise5) we know that $d \gamma = 0$ and $\delta \gamma = 0$. Then

$$
\begin{aligned}
\delta \omega &= \delta d \alpha + \delta \delta \beta + \delta \gamma = \delta d \alpha
\end{aligned}
$$

$$
\begin{aligned}
d \omega &= d d \alpha + d \delta \beta + d \gamma = d \delta \beta
\end{aligned}
$$