# Exercise2

Notice that norm function $g(x) = || x ||$ is convex, square function $f(x) = x^2$ is convex and non-decreasing on the range of $g(x)$, [0,$\infty$). Therefore, the composition $(f \circ g) (x) = || x ||^2$ is convex.

Then,

$$
\begin{aligned}
\eta || \nabla \phi_1 - X ||^2 + (1 - \eta) || \nabla \phi_2 - X ||^2 &\geq ||\eta \cdot (\nabla \phi_1 - X) + (1 - \eta) \cdot (\nabla \phi_2 - X) ||^2 \\
&= || \eta \nabla \phi_1 + (1 - \eta) \nabla \phi_2 - X ||^2 \\
\end{aligned}
$$

Take integration on the manifold $M$, we have

$$
\begin{aligned}
\eta \int_M || \nabla \phi_1 - X ||^2 d A + (1 - \eta) \int_M || \nabla \phi_2 - X ||^2 d A \geq \int_M || \eta \nabla \phi_1 + (1 - \eta) \nabla \phi_2 - X ||^2 d A
\end{aligned}
$$

$$
\begin{aligned}
\eta E(\phi_1) + (1 - \eta) E(\phi_2) \geq E( \eta \phi_1 + (1 - \eta) \phi_2 )
\end{aligned}
$$

which shows that $E(\phi)$ is convex.

# Exercise3

First expand the square norm,

$$
\begin{aligned}
|| \nabla \phi - X ||^2 = \langle \nabla \phi, \nabla \phi \rangle - 2 \langle \nabla \phi, X \rangle + \langle X, X \rangle
\end{aligned}
$$

Therefore,

$$
\begin{aligned}
E(\phi) &= \int_M || \nabla \phi - X ||^2 d A = \int_M \langle \nabla \phi, \nabla \phi \rangle - 2 \langle \nabla \phi, X \rangle + \langle X, X \rangle d A \\
&= \langle \langle \nabla \phi, \nabla \phi \rangle \rangle - 2 \langle \langle \nabla \phi, X \rangle \rangle + \langle \langle X, X \rangle \rangle \\
\end{aligned}
$$

According to [Green's first identity](https://en.wikipedia.org/wiki/Green%27s_identities#On_manifolds), the first part

$$
\begin{aligned}
\langle \langle \Delta \phi, \phi \rangle \rangle + \langle \langle \nabla \phi, \nabla \phi \rangle \rangle = \langle \langle N \cdot \nabla \phi, \phi \rangle \rangle_\partial = 0
\end{aligned}
$$

$$
\begin{aligned}
\langle \langle \nabla \phi, \nabla \phi \rangle \rangle = - \langle \langle \Delta \phi, \phi \rangle \rangle
\end{aligned}
$$

Similarly, the second part
$$
\begin{aligned}
\langle \langle \nabla \phi, X \rangle \rangle = - \langle \langle \phi, \nabla \cdot X \rangle \rangle
\end{aligned}
$$

Therefore,

$$
\begin{aligned}
E(\phi) &= - \langle \langle \Delta \phi, \phi \rangle \rangle + 2 \langle \langle \phi, \nabla \cdot X \rangle \rangle + || X ||^2 \\
\end{aligned}
$$

# Exercise4

$$
\begin{aligned}
E(\phi + \epsilon \psi) &= - \langle \langle \Delta (\phi + \epsilon \psi), \phi + \epsilon \psi \rangle \rangle + 2 \langle \langle \phi + \epsilon \psi, \nabla \cdot X \rangle \rangle + || X ||^2 \\
&= - \langle \langle \Delta \phi + \epsilon \Delta \psi, \phi + \epsilon \psi \rangle \rangle + 2 \langle \langle \phi + \epsilon \psi, \nabla \cdot X \rangle \rangle + || X ||^2 \\
&= - \langle \langle \Delta \phi, \phi \rangle \rangle - \epsilon \langle \langle \Delta \phi, \psi \rangle \rangle - \epsilon \langle \langle \Delta \psi, \phi \rangle \rangle - \epsilon^2 \langle \langle \Delta \psi, \psi \rangle \rangle + 2 \langle \langle \phi, \nabla \cdot X \rangle \rangle + 2 \epsilon \langle \langle \psi, \nabla \cdot X \rangle \rangle + || X ||^2 \\
&= E(\phi) - \epsilon \langle \langle \Delta \phi, \psi \rangle \rangle - \epsilon \langle \langle \Delta \psi, \phi \rangle \rangle - \epsilon^2 \langle \langle \Delta \psi, \psi \rangle \rangle + 2 \epsilon \langle \langle \psi, \nabla \cdot X \rangle \rangle
\end{aligned}
$$

Therefore,

$$
\begin{aligned}
D_\psi E(\phi) &= \lim_{\epsilon \to 0} \frac{E(\phi + \epsilon \psi) - E(\phi)}{\epsilon} \\
&= - \langle \langle \Delta \phi, \psi \rangle \rangle - \langle \langle \Delta \psi, \phi \rangle \rangle + 2 \langle \langle \psi, \nabla \cdot X \rangle \rangle \\
&= - 2 \langle \langle \Delta \phi, \psi \rangle \rangle + 2 \langle \langle \psi, \nabla \cdot X \rangle \rangle \\
&= 2 \langle \langle \psi, \nabla \cdot X - \Delta \phi \rangle \rangle
\end{aligned}
$$

# Exercise5

From [Exercise4](#exercise4) we have

$$
\begin{aligned}
D_\psi E(\phi) &= \langle \langle \psi, 2 (\nabla \cdot X - \Delta \phi) \rangle \rangle \\
&= \langle \langle \nabla E(\phi), \psi \rangle \rangle
\end{aligned}
$$

Therefore,

$$
\begin{aligned}
\nabla E(\phi) &= 2 (\nabla \cdot X - \Delta \phi)
\end{aligned}
$$

Set $\nabla E(\phi) = 0$, we have

$$
\begin{aligned}
\Delta \phi = \nabla \cdot X
\end{aligned}
$$

# Exercise6

Take integration over the dual cell of vertex $i$. According to the divergence theorem,

$$
\begin{aligned}
\int_\Omega \nabla \cdot X \ dA &= \int_{\partial \Omega} n \cdot X \ dl \\
&= \sum_{j} \Big(\frac{e_1}{| e_1 |} \cdot X_j \Big) l_1 +\Big(\frac{e_2}{| e_2 |} \cdot X_j \Big) l_2 \\
&= \sum_{j} \frac{l_1}{| e_1 |} e_1 \cdot X_j + \frac{l_2}{| e_2 |} e_2 \cdot X_j \\
&= \sum_{j} \frac{1}{2} \cot{\theta_1} (e_1 \cdot X_j) + \frac{1}{2} \cot{\theta_2} (e_2 \cdot X_j) \\
&= \frac{1}{2} \sum_{j} \cot{\theta_1} (e_1 \cdot X_j) + \cot{\theta_2} (e_2 \cdot X_j)
\end{aligned}
$$
