# Exercise1

1. $$v \wedge w = (e_1 + 2 e_2) \wedge (e_2 + 2 e_3) = e_1 \wedge e_2 + 2 e_1 \wedge e_3 + 2 e_2 \wedge e_2 + 4 e_2 \wedge e_3 = e_1 \wedge e_2 + 4 e_2 \wedge e_3 - 2 e_3 \wedge e_1$$
2. $$w \wedge v = (e_2 + 2 e_3) \wedge (e_1 + 2 e_2) = -e_1 \wedge e_2 - 4 e_2 \wedge e_3 + 2 e_3 \wedge e_1 = -(v \wedge w)$$
3. $$v \wedge v = (e_1 + 2 e_2) \wedge (e_1 + 2 e_2) = 0$$

# Exercise2

$$
\begin{aligned}
    \alpha_0 \wedge \alpha_1 \wedge \alpha_2 &= (e_1 + e_2) \wedge (e_1 + 2 e_2) \wedge (e_1 + 4 e_2) \\
    &= (e_1 \wedge e_1 + 2 e_1 \wedge e_2 + e_2 \wedge e_1 + 2 e_2 \wedge e_2) \wedge (e_1 + 4 e_2) \\
    &= (e_1 \wedge e_2) \wedge (e_1 + 4 e_2) \\
    &= e_1 \wedge e_2 \wedge e_1 + 4 e_1 \wedge e_2 \wedge e_2 \\
    &= 0
\end{aligned}
 $$

# Exercise3
$$
\begin{aligned}
    u \wedge v &= (e_1 + e_2 + e_3) \wedge (e_1 - e_2 + e_3) \\
    &= -e_1 \wedge e_2 + e_1 \wedge e_3 + e_2 \wedge e_1 + e_2 \wedge e_3 + e_3 \wedge e_1 - e_3 \wedge e_2 \\
    &= -2 e_1 \wedge e_2 + 2 e_2 \wedge e_3
\end{aligned}
$$

$$
\begin{aligned}
    u \times v &= (e_1 + e_2 + e_3) \times (e_1 - e_2 + e_3) \\
    &= -e_1 \times e_2 + e_1 \times e_3 + e_2 \times e_1 + e_2 \times e_3 + e_3 \times e_1 - e_3 \times e_2 \\
    &= -2e_3 + 2e_1
\end{aligned}
$$

# Exercise4

1. 
$$
\begin{aligned}
    u \wedge v + v \wedge w &= (e_1 + e_2 - e_3) \wedge (e_1 - e_2 + 2 e_3) + (e_1 - e_2 + 2 e_3) \wedge (3 e_1 + e_2) \\
    &= (-2 e_1 \wedge e_2 +  e_2 \wedge e_3 - 3 e_3 \wedge e_1) + (4 e_1 \wedge e_2 - 2 e_2 \wedge e_3 + 6 e_3 \wedge e_1) \\
    &= 2 e_1 \wedge e_2 - e_2 \wedge e_3 + 3 e_3 \wedge e_1
\end{aligned}
$$

2. 
$$
\begin{aligned}
    (u \wedge v) \wedge w &= (e_1 + e_2 - e_3) \wedge (e_1 - e_2 + 2 e_3) \wedge (3 e_1 + e_2) \\ 
    &= (-2 e_1 \wedge e_2 +  e_2 \wedge e_3 - 3 e_3 \wedge e_1) \wedge (3 e_1 + e_2) \\ 
    &= 3 e_1 \wedge e_2 \wedge e_3 - 3 e_1 \wedge e_2 \wedge e_3 \\
    &= 0
\end{aligned}
$$

# Exercise5
1. $$\star e_1 = e_2$$

2. $$\star e_1 = e_2 \wedge e_3$$

# Exercise6
1. 
$$
\begin{aligned}
    \star \alpha &= \star (e_1 + e_2 + e_3) = \star e_1 + \star e_2 + \star e_3 \\
    &= e_2 \wedge e_3 + e_3 \wedge e_1 + e_1 \wedge e_2
\end{aligned}
$$

$$
\begin{aligned}
    \star \beta &= \star (e_1 - e_2 + 2 e_3) = \star e_1 - \star e_2 + 2 \star e_3 \\
    &= e_2 \wedge e_3 - e_3 \wedge e_1 + 2 e_1 \wedge e_2
\end{aligned}
$$

2. 
$$
\begin{aligned}
    \star (\alpha \wedge \beta) &= \star [(e_1 + e_2 + e_3) \wedge (e_1 - e_2 + 2 e_3)] \\
    &= \star (-2e_1 \wedge e_2 + 3 e_2 \wedge e_3 - e_3 \wedge e_1) \\
    &= 3 e_1 - e_2 -2 e_3
\end{aligned}
$$

3. 
$$
\begin{aligned}
    (\star \alpha) \wedge (\star \beta) &= (e_2 \wedge e_3 + e_3 \wedge e_1 + e_1 \wedge e_2) \wedge (e_2 \wedge e_3 - e_3 \wedge e_1 + 2 e_1 \wedge e_2) \\
    &= 0
\end{aligned}
$$

# Exercise7
1.  Suppose $w = x e_1 + y e_2$, then
    $$
    \begin{aligned}
        \star w &= \star(x e_1 + y e_2) \\
        &= x \star e_1 + y \star e_2 \\
        &= -y e_1 + x e_2
    \end{aligned}
    $$

    Therefore,
    $$
    \begin{aligned}
        \star(\star w) &= \star(-y e_1 + x e_2) \\
        &= -y \star e_1 + x \star e_2 \\
        &= -x e_1 - y e_2 \\
        &= -w
    \end{aligned}
    $$

2.  Suppose $w = x e_1 + y e_2 + z e_3$, then
    $$
    \begin{aligned}
        \star w &= \star(x e_1 + y e_2 + z e_3) \\
        &= x \star e_1 + y \star e_2 + z e_3 \\
        &= x e_2 \wedge e_3 + y e_3 \wedge e_1 + z e_1 \wedge e_2
    \end{aligned}
    $$

    Therefore,
    $$
    \begin{aligned}
        \star(\star w) &= \star(x e_2 \wedge e_3 + y e_3 \wedge e_1 + z e_1 \wedge e_2) \\
        &= x \star(e_2 \wedge e_3) + y \star(e_3 \wedge e_1) + z \star(e_1 \wedge e_2) \\
        &= x e_1 + y e_2 + z e_3 \\
        &= w
    \end{aligned}
    $$

3.  (Use determinant to prove) 
    $$ \star(\star w) = (-1)^{n+1} w $$

4.  $$ \star(\star w) = (-1)^{k (n-1)} w $$

# Exercise8
1. 
$$
\begin{aligned}
    \alpha \wedge (\beta + \star \gamma) &= 2 e_3 \wedge [(e_1 - e_2) + \star (e_2 \wedge e_3)] \\
    &= 2 e_3 \wedge (e_1 - e_2 - e_1) \\
    &=-2 e_3 \wedge e_2 \\
    &= 2 e_1 
\end{aligned}
$$

2. 
$$
\begin{aligned}
    \star(\gamma \wedge \star (\alpha \wedge \beta)) &= \star((e_2 \wedge e_3) \wedge \star (2 e_3 \wedge (e_1 - e_2))) \\
    &= \star((e_2 \wedge e_3) \wedge (2 e_1 + 2 e_2)) \\
    &= \star(2 e_2 \wedge e_3 \wedge e_1) \\
    &= 2
\end{aligned}
$$

# Exercise9

1. 
$$ \alpha = 2z \ dx + 3 x^2 \ dy + 5 \cos(y) \ dz $$

2. 
$$
\begin{aligned}
    \alpha (U) &= 6 z + 6 x^2 + 5 \cos(y) \\
    \alpha (U)_p &= 6 \times 3 + 6 \times 1^2 + 5 \cos(2) = 24 + 5 \cos(2)
\end{aligned}
$$

3. 
$$ -\alpha = -2z \ dx - 3 x^2 \ dy - 5 \cos(y) \ dz $$

# Exercise10

1. $\alpha (U)$ is a 0-form.

2. 
$$
\begin{aligned}
    \alpha (U) &= 2 x \\
    \alpha (V) &= x^2 y \\
    \beta (U) &= 1 + x \\
    \beta (V) &= 4 \\
\end{aligned}
$$

3. 
$$
\begin{aligned}
    \alpha \wedge \beta (U, V) &= \alpha (U) \beta (V) - \alpha (V) \beta (U) \\
    &= 2 x \times 4 - x^2 y \times (1 + x) \\
    &= - x^3 y - x^2 y + 8 x
\end{aligned}
$$

4. 
$$
\begin{aligned}
    \alpha \wedge \beta (V, U) &= \alpha (V) \beta (U) - \alpha (U) \beta (V) \\
    &= x^3 y + x^2 y - 8 x
\end{aligned}
$$

# Exercise11

1. 
$$
\begin{aligned}
    (\star [d (e^y dx + \sin(z) dz)]) \wedge dz &= (\star [-e^y dx \wedge dy]) \wedge dz \\
    &= -e^y dz \wedge dz \\
    &= 0
\end{aligned}
$$

2. 
$$
\begin{aligned}
    d[\star (d(dx \wedge z^2 dy)) + \star (xyz \ dx \wedge dz \wedge dy)] &= d[\star (-dx \wedge d(z^2 dy)) - xyz] \\
    &= d[\star (2z \ dx \wedge dy \wedge dz) - xyz] \\
    &= d[2z - xyz] \\
    &= 2 dz - yz dx - xz \ dy - xy \ dz \\
    &= - yz dx - xz \ dy + (2 - xy) \ dz
\end{aligned}
$$

# Exercise12

1. If $\alpha$ is a 0-form, then $\star \alpha$ is a $n$-form and $d(\star \alpha)$ is 0. So $\delta \alpha = 0$.

2. If $\alpha$ is a $k$-form, then $\star \alpha$ is a $(n-k)$-form and $d(\star \alpha)$ is a $(n-k+1)$-form. So $\delta \alpha = \star (d(\star \alpha))$ is a $(k - 1)$-form.

3. 
$$
\begin{aligned}
    \delta \alpha &= \star (d(\star \alpha)) = \star (d(\star (e^y dx + (x + y)^2 dy))) \\
    &= \star (d(e^y dy - (x + y)^2 dx)) \\
    &= \star (-2(x + y) dy \wedge dx) \\
    &= 2 (x + y)
\end{aligned}
$$

# Exercise13

1. If $\alpha$ is a 0-form, then $\star \alpha$ is a $n$-form and $d(\star \alpha)$ is 0. Therefore, $d \star d \star \alpha = 0$.

2. $$ \Delta \phi =  4 $$

3. 
$$
\begin{aligned}
    \Delta \phi &= \star d \star d \phi + d \star d \star \phi = \star d \star d \phi \\
    &= \star d \star (y \ dx + (x + 4y) \ dy) \\
    &= \star d (y dy - (x + 4y) dx) \\
    &= \star (-4 dy \wedge dx) \\
    &= 4
\end{aligned}
$$

4. 
$$
\begin{aligned}
    \Delta \alpha &= \star d \star d \alpha + d \star d \star \alpha
\end{aligned}
$$

$$ 
\begin{aligned}
\star d \star d \alpha &= \star d \star d(x dx + z dy - y dz) \\
&= \star d \star (-2 dy \wedge dz) \\
&= \star d (-2 dx) \\
&= 0
\end{aligned}
$$

$$ 
\begin{aligned}
d \star d \star \alpha &= d \star d \star (x dx + z dy - y dz) \\
&= d \star d (x dy \wedge dz + z dz \wedge dx - y dx \wedge dy) \\
&= d \star (dx \wedge dy \wedge dz) \\
&= 0
\end{aligned}
$$

Therefore, 
$$
\begin{aligned}
    \Delta \alpha &= \star d \star d \alpha + d \star d \star \alpha = 0
\end{aligned}
$$

